WIP: new equivalence relations, use size for recursion

src/ExpEquiv.v
@@ -1,4 +1,7 @@
-Require Import ExpSemantics.
+Require Export ExpSemantics.
+Export PeanoNat.
+Export Relations.Relations.
+Export Classes.RelationClasses.
 
 Import ListNotations.
 
@@ -37,56 +40,757 @@ Notation "C [[ e ]]" := (fill_boxes e C) (at level 30).
 
 Compute (CBox) [[ ELit 1 ]].
 
-(*
-Inductive value_equivalent : Exp -> Exp -> Prop :=
-| vrefl v : is_value v -> value_equivalent v v
-| vclos : forall v1 v2, is_value v1 -> is_value v2 ->
-   (forall vals fs, | fs, EApp (EFun vl e) vals | -->* |fs, v1 |) .
+Inductive Value : Set :=
+| VLit (z : Z)
+| VFun (env : list ((Var + FunctionIdentifier) * Value)) (vl : list Var) (b : Exp)
+| VRecFun (env : list ((Var + FunctionIdentifier) * Value)) (f : FunctionIdentifier) (vl : list Var) (b : Exp).
 
-Definition ctx_preorder (e1 e2 : Exp) : Prop :=
-  forall (C : Context) (* (fs : FrameStack)  *) (v1 v2 : Exp),
-  is_value v1 -> is_value v2 -> value_equivalent v1 v2
-->
-  | [], C[[e1]] | -->* | [], v1 | -> | [], C[[e2]] | -->* | [], v2 |
+
+Definition Environment : Set := list ((Var + FunctionIdentifier) * Value).
+
+
+(* The equality of function signatures *)
+  Definition funid_eqb (v1 v2 : FunctionIdentifier) : bool :=
+  match v1, v2 with
+  | (fid1, num1), (fid2, num2) => eqb fid1 fid2 && Nat.eqb num1 num2
+  end.
+
+  (* Extended equality between functions and vars *)
+  Definition var_funid_eqb (v1 v2 : Var + FunctionIdentifier) : bool :=
+  match v1, v2 with
+  | inl s1, inl s2 => eqb s1 s2
+  | inr f1, inr f2 => funid_eqb f1 f2
+  | _, _ => false
+  end.
+
+(** Get *)
+Fixpoint get_value (env : Environment) (key : (Var + FunctionIdentifier)) 
+   : option Value :=
+match env with
+| [ ] => None
+| (k,v)::xs => if var_funid_eqb key k then Some v else get_value xs key
+end.
+
+(** Insert *)
+Fixpoint insert_value (env : Environment) (key : (Var + FunctionIdentifier)) 
+   (value : Value) : Environment :=
+match env with
+  | [] => [(key, value)]
+  | (k,v)::xs => if var_funid_eqb k key then (key,value)::xs else (k,v)::(insert_value xs key value)
+end.
+
+(** Add bindings with two lists *)
+Fixpoint append_vars_to_env (vl : list Var) (el : list Value) (d : Environment) 
+   : Environment :=
+match vl, el with
+| [], [] => d
+| v::vs, e::es => append_vars_to_env vs es (insert_value d (inl v) e)
+| _, _ => d (** length check needed *)
+end.
+
+Inductive ResultType {T : Set} : Set :=
+| Timeout
+| Fail
+| Res (v : T)
 .
 
-Definition ctx_equivalent (e1 e2 : Exp) : Prop :=
-  ctx_preorder e1 e2 /\ ctx_preorder e2 e1
+Fixpoint eval_list (f : Exp -> @ResultType Value) (l : list Exp) : @ResultType (list Value) :=
+match l with
+| [] => Res []
+| x::xs => match f x with
+           | Res v => match eval_list f xs with
+                       | Res vs => Res (v::vs)
+                       | r => r
+                       end
+           | Fail => Fail
+           | Timeout => Timeout
+           end
+end.
+
+Fixpoint eval_env (clock : nat) (env : Environment) (e : Exp) : @ResultType Value :=
+match clock with
+| 0 => Timeout
+| S n => match e with
+         | ELit l => Res (VLit l)
+         | EVar v => match get_value env (inl v) with
+                     | Some val => Res val
+                     | None => Fail
+                     end
+         | EFunId f => match get_value env (inr f) with
+                       | Some val => Res val
+                       | None => Fail
+                       end
+         | EFun vl e => Res (VFun env vl e)
+         | ERecFun f vl e => Res (VRecFun env f vl e)
+         | EApp exp l => match eval_env n env exp with
+                         (** In Core Erlang this check only happens later *)
+                         | Res (VFun env' vl e) =>
+                            (* This would be better with Monads *)
+                            let vres := eval_list (eval_env n env) l in
+                               match vres with
+                               | Res vals => eval_env n (append_vars_to_env vl vals env') e
+                               | Fail => Fail
+                               | Timeout => Timeout
+                               end
+                         | Res (VRecFun env' f vl e) =>
+                            let vres := eval_list (eval_env n env) l in
+                               match vres with
+                               | Res vals => eval_env n (append_vars_to_env vl vals (insert_value env' (inr f) (VRecFun env' f vl e))) e
+                               | Fail => Fail
+                               | Timeout => Timeout
+                               end
+                         | Res _  => Fail
+                         | r => r
+                         end
+         | ELet v e1 e2 => match eval_env n env e1 with
+                           | Res val => eval_env n (insert_value env (inl v) val) e2
+                           | r      => r
+                           end
+         | ELetRec f vl b e => eval_env n (insert_value env (inr f) (VRecFun env f vl b)) e
+         | EPlus e1 e2 => 
+            match eval_env n env e1, eval_env n env e2 with
+            | Res (VLit n), Res (VLit m) => Res (VLit (n + m))
+            | Res _, Res _ => Fail
+            | Res _, r => r
+            | r, _     => r
+            end
+         | EIf e1 e2 e3 =>
+            match eval_env n env e1 with
+            | Res (VLit 0) => eval_env n env e2
+            | Res _        => eval_env n env e3
+            | r            => r
+            end
+        end
+end.
+
+Definition make_exp (v : Value) : Exp :=
+match v with
+ | VLit z => ELit z
+ | VFun env vl b => EFun vl b
+ | VRecFun env f vl b => ERecFun f vl b
+end.
+
+Definition make_exps (l : list Value) : list Exp := map make_exp l.
+
+Definition terminating (e : Exp) (env : Environment) : Prop :=
+  exists v clock, eval_env clock env e = Res v
 .
 
-Lemma ctx_preorder_refl :
-  forall e, ctx_preorder e e.
-Proof. firstorder. Qed.
+Axiom bigger_clock :
+  forall env e clock v clock', clock' >= clock ->
+   eval_env clock env e = Res v ->
+   eval_env clock' env e = Res v.
 
-Lemma ctx_preorder_trans :
-  forall e1 e2 e3, ctx_preorder e1 e2 -> ctx_preorder e2 e3
+(* TODO: fix this with typing *)
+(* Unset Positivity Checking. *)
+
+Inductive val_rel : relation Value :=
+(* | lit_rel z z' : 
+  z = z' -> val_rel (VLit z) (VLit z') *)
+| refl_rel v : val_rel v v
+| clos_rel vl env b vl' env' b' :
+  length vl = length vl' ->
+  (forall vals, length vals = length vl -> (*1 vals2, list_rel vals1 vals2 (* length vals1 = length vl -> length vals2 = length vl' ->
+    (forall i, i < length vl -> val_rel (nth i vals1 (VLit 0)) (nth i vals2 (VLit 0)) )*) ->*)
+  exp_rel (append_vars_to_env vl vals env) (append_vars_to_env vl' vals env') b b')
 ->
-  ctx_preorder e1 e3.
-Proof. firstorder. Qed.
-
-Lemma ctx_eq_refl :
-  forall e, ctx_equivalent e e.
-Proof. firstorder. Qed.
-
-Lemma ctx_eq_sym :
-  forall e1 e2, ctx_equivalent e1 e2 -> ctx_equivalent e2 e1.
-Proof. firstorder. Qed.
-
-Lemma ctx_eq_trans :
-  forall e1 e2 e3,
-  ctx_equivalent e1 e2 -> ctx_equivalent e2 e3
+  val_rel (VFun env vl b) (VFun env' vl' b')
+| rec_clos_rel f vl env b f' vl' env' b' :
+  length vl = length vl' ->
+  (forall vals, length vals = length vl -> (*1 vals2, length vals1 = length vl -> length vals2 = length vl' ->
+    (forall i, i < length vl -> val_rel (nth i vals1 (VLit 0)) (nth i vals2 (VLit 0))) ->*)
+  exp_rel (append_vars_to_env vl vals (insert_value env (inr f) (VRecFun env f vl b))) 
+          (append_vars_to_env vl' vals (insert_value env' (inr f') (VRecFun env' f' vl' b'))) b b')
 ->
-  ctx_equivalent e1 e3.
-Proof. firstorder. Qed.
-
-Theorem relations_simulation :
-  exists R : Exp -> Exp -> Prop,
-  forall (e1 e2 : Exp) (v1 v2 : Exp),
-  (forall fs : FrameStack, | fs, e1 | -->* | fs, v1 |) -> is_value v1 ->
-  (forall fs : FrameStack, | fs, e2 | -->* | fs, v2 |) -> is_value v2 ->
-  R v1 v2 
+  val_rel (VRecFun env f vl b) (VRecFun env' f' vl' b')
+with exp_rel : Environment -> Environment -> Exp -> Exp -> Prop :=
+| exp_rel_cons env env' e1 e2:
+  (terminating e1 env <-> terminating e2 env') ->
+  (forall v1 v2 clock,
+      eval_env clock env e1 = Res v1 /\
+      eval_env clock env' e2 = Res v2 ->
+      val_rel v1 v2)
 ->
-  R e1 e2.
+  exp_rel env env' e1 e2
+(* | exp_rel_cons env env' e1 e2:
+  (forall clock,
+      match eval_env clock env e1, eval_env clock env' e2 with
+      | Res v1, Res v2 => val_rel v1 v2
+      | _, _ => True
+      end)
+->
+  exp_rel env env' e1 e2 *)
+(* | exp_rel_cons env env' e1 e2:
+  (forall v1 v2 clock,
+    val_rel v1 v2 ->
+     eval_env clock env e1 = Res v1 <-> (* exists clock needed, cannot be used to reason about divergent programs *)
+     eval_env clock env' e2 = Res v2)
+->
+  exp_rel env env' e1 e2 *)
+(* with list_rel : list Value -> list Value -> Prop :=
+| nil_rel : list_rel [] []
+| cons_rel x y xs ys : val_rel x y -> list_rel ys ys -> list_rel (x::xs) (y::ys) *)
+.
+
+Set Positivity Checking.
+
+Scheme ind11 := Induction for val_rel Sort Prop
+with ind22 := Induction for exp_rel Sort Prop
+(* with ind33 := Induction for list_rel Sort Prop *).
+
+Check ind22.
+
+Combined Scheme exp_rel_ind2 from ind11, ind22(* , ind33 *).
+
+Check exp_rel_ind2.
+
+Goal forall x (P : Value -> Prop),
+  match x with
+  | Res y => P y
+  | _     => True
+  end
+  <->
+  (forall y, x = Res y -> P y).
+Proof.
+  split; intros.
+  destruct x; inversion H0. subst. auto.
+  destruct x; auto.
+Qed.
+
+Goal forall x y (P : Value -> Value -> Prop),
+  match x, y with
+  | Res x', Res y' => P x' y'
+  | _ , _          => True
+  end
+  <->
+  (forall x' y', x = Res x' /\ y = Res y' -> P x' y').
+Proof.
+  split; intros.
+  * destruct H0. subst. auto.
+  * destruct x, y; auto.
+Qed.
+
+Definition equiv_env : relation Environment :=
+ fun env env' =>
+  length env = length env' /\
+  forall i, i < length env -> val_rel (snd (nth i env (inl "X"%string, VLit 0))) (snd (nth i env' (inl "X"%string, VLit 0))).
+
+Definition equiv_rel : relation Exp := fun e1 e2 =>
+  forall env env', equiv_env env env' -> exp_rel env env' e1 e2
+.
+
+Theorem val_rel_refl :
+  Reflexive val_rel.
+Proof.
+  constructor.
+Qed.
+
+Theorem exp_rel_refl :
+  forall env, Reflexive (exp_rel env env).
+Proof.
+  intros. constructor.
+  * split; auto.
+  * intros. destruct H. rewrite H in H0. inversion H0. constructor.
+Qed.
+
+Theorem equiv_env_eval :
+  forall clock e env env' v, equiv_env env env'
+->
+  eval_env clock env e = Res v
+->
+  exists v', eval_env clock env' e = Res v' /\ val_rel v v'.
+Proof.
+  induction clock; intros.
+  * inversion H0.
+  * destruct e.
+    - simpl in H0. inversion H0.
+Admitted.
+
+Corollary equiv_env_term :
+  forall env env' e, equiv_env env env' -> terminating e env -> terminating e env'.
+Proof.
+  intros. unfold terminating in *. destruct H0, H0. eapply equiv_env_eval in H0. 2: exact H. destruct H0, H0.
+  eexists. exists x0. exact H0.
+Qed.
+
+Theorem val_rel_sym :
+  (forall v1 v2, val_rel v1 v2 -> val_rel v2 v1)
+/\
+  (forall env env' v1 v2, exp_rel env env' v1 v2 -> exp_rel env' env v2 v1)
+(* /\
+  (forall l1 l2, list_rel l1 l2 -> list_rel l2 l1) *).
+Proof.
+  intros. apply exp_rel_ind2.
+  * constructor.
+  * constructor. symmetry. auto. intros. apply H. lia.
+  * constructor. symmetry. auto. intros. apply H. lia.
+  * intros. constructor.
+    - destruct i. split; auto.
+    - intros. eapply H. destruct H0. split. exact e0. exact e.
+Qed. 
+
+Theorem equiv_env_refl :
+  forall env, equiv_env env env.
+Proof. firstorder. constructor. Qed.
+
+Theorem equiv_env_sym :
+  forall env env', equiv_env env env' -> equiv_env env' env.
+Proof.
+  firstorder. apply val_rel_sym. apply H0. lia.
+Qed.
+
+Theorem equiv_rel_refl :
+  forall e, equiv_rel e e.
+Proof.
+  econstructor. intros.
+  * split; apply equiv_env_term; auto. apply equiv_env_sym. auto.
+  * intros. destruct H0. epose (equiv_env_eval _ _ _ _ _ H H0). destruct e0, H2. rewrite H1 in H2.
+    inversion H2. subst. auto.
+Qed.
+
+Check exp_rel_ind.
+
+Theorem equiv_rel_sym:
+  forall e1 e2, equiv_rel e1 e2 -> equiv_rel e2 e1.
+Proof.
+  unfold equiv_rel in *. intros. apply val_rel_sym. eapply H. apply equiv_env_sym. auto.
+Qed.
+
+Theorem val_rel_trans :
+  (forall v1 v2, val_rel v1 v2 -> (forall v3, val_rel v2 v3 -> val_rel v1 v3))
+/\
+  (forall env1 env2 e1 e2, exp_rel env1 env2 e1 e2 -> (forall env3 e3, exp_rel env2 env3 e2 e3 -> exp_rel env1 env3 e1 e3)).
+Proof.
+  apply exp_rel_ind2; intros.
+  * auto.
+  * inversion H0.
+    - subst. constructor. lia. intros. apply H. lia. apply exp_rel_refl.
+    - subst. constructor. lia. intros. apply H. lia. apply H6. lia.
+  * inversion H0.
+    - subst. constructor. lia. intros. apply H. lia. apply exp_rel_refl.
+    - subst. constructor. lia. intros. apply H. lia. apply H7. lia.
+  * inversion H0. subst. constructor.
+    - eapply iff_trans. exact i. auto.
+    - intros. destruct H3.
+      apply ex_intro with (x := clock) in H3 as Hex. apply ex_intro with (x := v1) in Hex.
+      apply ex_intro with (x := clock) in H4 as H0ex. apply ex_intro with (x := v2) in H0ex.
+      apply i in Hex. apply H1 in H0ex. destruct Hex, H0ex, H5, H6.
+      apply bigger_clock with (clock' := clock + x1) in H3.
+      apply bigger_clock with (clock' := clock + x1) in H5.
+      apply bigger_clock with (clock' := clock + x1) in H4. all: try lia.
+      pose (H v1 x _ (conj H3 H5)). apply v0.
+      destruct H0.
+      epose (H7 _ _ _ (conj H5 _)). exact v3. Unshelve. auto.
+Qed.
+
+Theorem equiv_rel_trans :
+  forall e1 e2 e3, equiv_rel e1 e2 -> equiv_rel e2 e3 -> equiv_rel e1 e3.
+Proof.
+  unfold equiv_rel. intros. eapply val_rel_trans. eapply H. exact H1. (* I can choose equiv_env for e2 *)
+  eapply H0. apply equiv_env_refl.
+Qed.
+
+Tactic Notation "start_equiv" := unfold equiv_rel; intros; constructor.
+Tactic Notation "prove_term" := split; intros; eexists; exists 1000; simpl; reflexivity.
+
+Goal
+  equiv_rel (ELit 5) (EPlus (ELit 5) (ELit 0)).
+Proof.
+  start_equiv. prove_term.
+  * intros. destruct H0. destruct clock; inversion H0.
+    destruct clock; inversion H1. constructor.
+Qed.
+
+Goal
+  equiv_rel (EFun [] (ELit 1)) (EFun [] (EPlus (ELit 0) (ELit 1))).
+Proof.
+  start_equiv. prove_term.
+  intros. destruct H0. destruct clock; inversion H0. inversion H1. subst.
+  constructor. intros. auto. simpl.
+  intros. apply length_zero_iff_nil in H2. subst.
+  constructor. prove_term.
+  intros. destruct H2.
+  destruct clock0; inversion H2. destruct clock0; inversion H3. constructor.
+Qed.
+
+Proposition var_funid_eqb_neq (v0 v : Var + FunctionIdentifier):
+    var_funid_eqb v0 v = false <-> v0 <> v.
+  Proof.
+    split; intros.
+    { destruct v0, v.
+      * simpl in *. apply eqb_neq in H. unfold not in *. intros. apply H. inversion H0. reflexivity.
+      * unfold not. intro. inversion H0.
+      * unfold not. intro. inversion H0.
+      * destruct f, f0. simpl in H. apply Bool.andb_false_iff in H. inversion H.
+        - apply eqb_neq in H0. unfold not in *. intro. apply H0. inversion H1. reflexivity.
+        - apply Nat.eqb_neq in H0. unfold not in *. intro. apply H0. inversion H1. reflexivity.
+    }
+    { destruct v0, v.
+      * simpl in *. apply eqb_neq. unfold not in *. intro. apply H. subst. reflexivity.
+      * simpl. reflexivity.
+      * simpl. reflexivity.
+      * simpl. destruct f, f0. simpl. apply Bool.andb_false_iff.
+        unfold not in H. case_eq ((s =? s0)%string); intros.
+        - right. apply eqb_eq in H0. apply Nat.eqb_neq. unfold not. intro. apply H. subst. reflexivity.
+        - left. reflexivity.
+    }
+  Qed.
+
+  Proposition var_funid_eqb_refl (var : Var + FunctionIdentifier) :
+  var_funid_eqb var var = true.
+  Proof.
+    destruct var.
+    * simpl. apply eqb_refl.
+    * destruct f. simpl. rewrite eqb_refl, Nat.eqb_refl. simpl. reflexivity.
+  Qed.
+
+  Proposition var_funid_eqb_sym (v1 v2 : Var + FunctionIdentifier) :
+    var_funid_eqb v1 v2 = var_funid_eqb v2 v1.
+  Proof.
+    destruct v1, v2.
+    * simpl. rewrite eqb_sym. reflexivity.
+    * simpl. reflexivity.
+    * simpl. reflexivity.
+    * simpl. destruct f, f0. simpl. rewrite eqb_sym, Nat.eqb_sym. reflexivity.
+  Qed.
+  
+  Proposition var_funid_eqb_eq (v0 v : Var + FunctionIdentifier):
+    var_funid_eqb v0 v = true <-> v0 = v.
+  Proof.
+    intros. split; intros.
+    { destruct v0, v.
+      * inversion H. apply eqb_eq in H1. subst. reflexivity.
+      * inversion H.
+      * inversion H.
+      * inversion H. destruct f, f0. inversion H1. apply Bool.andb_true_iff in H2. inversion H2.
+        apply eqb_eq in H0. apply Nat.eqb_eq in H3. subst. reflexivity.
+    }
+    { destruct v, v0.
+      * inversion H. subst. simpl. apply eqb_refl.
+      * inversion H.
+      * inversion H.
+      * inversion H. simpl. destruct f. simpl. rewrite eqb_refl, Nat.eqb_refl. simpl. reflexivity.
+    }
+  Qed.
+
+Proposition get_value_here (env : Environment) (var : Var + FunctionIdentifier) (val : Value):
+get_value (insert_value env var val) var = Some val.
+Proof.
+  induction env.
+  * simpl. rewrite var_funid_eqb_refl. reflexivity.
+  * simpl. destruct a. case_eq (var_funid_eqb s var); intro.
+    - simpl. rewrite var_funid_eqb_refl. reflexivity.
+    - simpl. rewrite var_funid_eqb_sym, H. assumption.
+Qed.
+
+(** Previous append result *)
+Proposition get_value_there (env : Environment) (var var' : Var + FunctionIdentifier) 
+     (val : Value):
+var <> var' ->
+get_value (insert_value env var val) var' = get_value env var'.
+Proof.
+  intro. induction env.
+  * simpl. apply var_funid_eqb_neq in H. rewrite var_funid_eqb_sym in H. rewrite H. reflexivity.
+  * simpl. destruct a. case_eq (var_funid_eqb s var); intro.
+    - apply var_funid_eqb_eq in H0. assert (var <> var'). auto. rewrite <- H0 in H.
+      apply var_funid_eqb_neq in H. rewrite var_funid_eqb_sym in H. rewrite H. simpl. apply var_funid_eqb_neq in H1.
+      rewrite var_funid_eqb_sym in H1. rewrite H1. reflexivity.
+    - simpl. case_eq (var_funid_eqb var' s); intros.
+      + reflexivity.
+      + apply IHenv.
+Qed.
+
+(* equivalent, substitutional semantics would be better *)
+Lemma foo env x :
+  eval_env (S (S (S (S (S (S (S (S (S x))))))))) env (sum 2) = Res (VLit 3).
+Proof.
+  remember (S (S (S (S (S (S x)))))) as xx. simpl.
+  rewrite get_value_here. rewrite Heqxx.
+  remember (S (S (S x))) as xxx. simpl. rewrite get_value_here.
+  rewrite get_value_there, get_value_here. 2: congruence. rewrite Heqxxx. simpl.
+  rewrite get_value_here, get_value_here.
+  rewrite get_value_there, get_value_here. 2: congruence. simpl.
+Admitted.
+
+Goal equiv_rel (sum 2) (ELit 3).
+Proof.
+  start_equiv. unfold sum.
+  split; intros. eexists. exists 10. reflexivity.
+  eexists. eexists. apply foo.
+  intros. destruct H. destruct clock; inversion H0. subst.
+Admitted.
+
+
+
+(** Congruence *)
+
+Ltac break_match_hyp :=
+match goal with
+| [ H : context [ match ?X with _=>_ end ] |- _] =>
+     match type of X with
+     | sumbool _ _=>destruct X
+     | _=>destruct X eqn:? 
+     end 
+end.
+
+Ltac break_match_goal :=
+match goal with
+| [ |- context [ match ?X with _=>_ end ] ] => 
+    match type of X with
+    | sumbool _ _ => destruct X
+    | _ => destruct X eqn:?
+    end
+end.
+
+Theorem equiv_env_insert :
+  forall env env',
+  equiv_env env env' ->
+  forall var v v', val_rel v v' -> equiv_env (insert_value env var v) (insert_value env' var v').
 Proof.
 
-Admitted.*)
+Admitted.
+
+Theorem equiv_env_app vars :
+  forall vals env env',
+  equiv_env env env' -> equiv_env (append_vars_to_env vars vals env) (append_vars_to_env vars vals env').
+Proof.
+  induction vars; intros.
+  * simpl. destruct vals; auto.
+  * simpl. destruct vals; auto. apply IHvars. apply equiv_env_insert; auto. constructor.
+Qed.
+
+
+Theorem equiv_rel_cong :
+  forall (C : Context) (e1 e2 : Exp),
+  equiv_rel e1 e2
+->
+  equiv_rel (C[[e1]]) (C[[e2]]).
+Proof.
+  induction C; intros.
+  * simpl. auto.
+  * simpl. constructor. prove_term.
+    intros. destruct H1. destruct clock; inversion H1. inversion H2. constructor.
+  * simpl. constructor.
+    - split; intros; eapply equiv_env_term; try exact H0. 2: exact (equiv_env_sym _ _ H0). auto. auto.
+    - intros. destruct H1.
+      pose (equiv_env_eval _ _ _ _ _ H0 H1). destruct e, H3. rewrite H3 in H2. inversion H2. subst. auto.
+  * simpl. constructor.
+    - split; intros; eapply equiv_env_term; try exact H0. 2: exact (equiv_env_sym _ _ H0). auto. auto.
+    - intros. destruct H1.
+      pose (equiv_env_eval _ _ _ _ _ H0 H1). destruct e, H3. rewrite H3 in H2. inversion H2. subst. auto.
+  * constructor. prove_term.
+    intros. destruct H1. destruct clock; inversion H1. inversion H2.
+    constructor. auto.
+    intros. apply IHC. exact H. apply equiv_env_app. auto.
+  * constructor. prove_term.
+    intros. destruct H1. destruct clock; inversion H1. inversion H2. (* cofix alma. *) (** possible coinduction needed *)
+    (* TODO: OR, which is better: finite unfolding *)
+    constructor. auto.
+    intros. (* constructor. *) apply IHC; auto. apply equiv_env_app. apply equiv_env_insert. auto.
+    admit.
+  * admit. (* wrong induction is generated for app, hand written is needed *)
+  * simpl. pose (IHC1 e1 e2 H). unfold equiv_rel in e. constructor.
+    - split; intros; destruct H1, H1, x0; inversion H1; break_match_hyp; try congruence.
+      pose (e _ _ H0). remember e0 as C1HYP. clear e0 HeqC1HYP e. inversion C1HYP. subst.
+      destruct H2.
+      eexists. exists (S x0).
+      simpl.
+
+Admitted.
+
+
+(*
+F := fun(X, Y) -> X(Y)
+
+F(fun(X) -> X, 1)
+F(fun(X) -> X + 1 - 1, 1) 
+*)
+
+(**
+
+(** Two events are A-related if they agree on all V-related values. *)
+Definition A_rel' (τ : Ty) (V_rel_τ : relation (val τ)) : relation (Event (val τ)) :=
+  fun A0 A1 =>
+    forall v0 v1 (Hv : V_rel_τ v0 v1),
+      (A0 v0 = (* iff *) A1 v1).
+Inductive val_rel : Value -> Value -> Prop :=
+| refl_rel v : val_rel v v
+| clos_rel vl env b vl' env' b' :
+  length vl = length vl' ->
+  (forall vals, length vals = length vl ->
+  exp_rel (append_vars_to_env vl vals env) (append_vars_to_env vl' vals env') b b')
+->
+  val_rel (VFun env vl b) (VFun env' vl' b')
+| rec_clos_rel f vl env b f' vl' env' b' :
+  length vl = length vl' ->
+  (forall vals, length vals = length vl ->
+  exp_rel (append_vars_to_env vl vals (insert_value env (inr f) (VRecFun env f vl b))) (append_vars_to_env vl' vals (insert_value env' (inr f') (VRecFun env' f' vl' b'))) b b')
+->
+  val_rel (VRecFun env f vl b) (VRecFun env' f' vl' b')
+with exp_rel : Environment -> Environment -> Exp -> Exp -> Prop :=
+| exp_rel_cons env env' e1 e2:
+  (terminating e1 env <-> terminating e2 env') ->
+  (forall v1 v2 clock,
+      eval_env clock env e1 = Res v1 /\
+      eval_env clock env' e2 = Res v2 ->
+      val_rel v1 v2)
+->
+  exp_rel env env' e1 e2
+.
+*)
+
+(*
+(** Two closed expressions are E-related if their value measures agree for all
+    A-related events. *)
+Definition E_rel' (τ : Ty) (V_rel_τ : relation (val τ)) : relation (expr · τ) :=
+  fun e0 e1 =>
+    forall A0 A1 (HA : A_rel' τ V_rel_τ A0 A1),
+      μ e0 A0 = μ e1 A1.*)
+
+(* Future work, based on https://github.com/cobbal/ppl-ctx-equiv-coq 
+  Trick: avoid positivity check by using typing
+*)
+
+Definition E_rel (V_rel : relation Value) (env env' : Environment) (e1 e2 : Exp) : Prop :=
+  ((terminating e1 env) <-> (terminating e2 env')) /\
+  (forall clock v1 v2,
+    eval_env clock env e1 = Res v1 /\
+    eval_env clock env e2 = Res v2 ->
+    V_rel v1 v2)
+.
+
+Definition V_rel_refl : relation Value := eq.
+Inductive V_rel_fun (valr : relation Value) : relation Value :=
+| clos_rel2 vl env b vl' env' b' :
+  length vl = length vl' ->
+  (forall vals1 vals2, length vals1 = length vl -> length vals2 = length vl' ->
+    (forall i, i < length vl -> valr (nth i vals1 (VLit 0)) (nth i vals2 (VLit 0))) ->
+  E_rel valr (append_vars_to_env vl vals1 env) (append_vars_to_env vl' vals2 env') b b')
+->
+  V_rel_fun valr (VFun env vl b) (VFun env' vl' b')
+(** TODO: recfun *)
+
+.
+
+(* Unset Positivity Checking. *)
+
+(* THe problem is not with endlessly recursive closures, because:
+  - their type would be a -> b, but b will not be extended! e.g. fun f X -> f X 
+                                     this is an application, not a closure  ^^^^
+  Probematic:
+  fun X -> fun X -> fun X -> .... <- however, this will be finite, because terms are finite
+  thus, we can take a natural number to measure the size instead of typing
+    ~> this number is decreased by applications, and increased by function definitions
+    - Idea: it should be the size of the term?
+*)
+
+(* Inductive v_rel : relation Value :=
+| rel_v v1 v2 : V_rel_refl v1 v2 -> v_rel v1 v2
+| rel_clos env env' vl vl' b b' : V_rel_fun v_rel (VFun env vl b) (VFun env' vl' b')
+  ->
+    v_rel (VFun env vl b) (VFun env' vl' b')
+.*)
+
+Fixpoint v_rel (n : nat) : relation Value :=
+fun v1 v2 =>
+match n with
+| 0 => True
+| S n' =>
+  match v1, v2 with
+  | VLit _, VLit _ => V_rel_refl v1 v2
+  | VFun _ _ _, VFun _ _ _ => V_rel_fun (v_rel n') v1 v2
+  | _, _ => False
+  end
+end.
+
+(* Set Positivity Checking. *)
+
+(* Fixpoint v_rel (v1 v2 : Value) : Prop :=
+match m with
+| Int => V_rel_refl v1 v2
+| Fun a b => V_rel_fun (v_rel a) (v_rel b) v1 v2
+end. *)
+
+Fixpoint size (e : Exp) : nat :=
+match e with
+ | ELit l => 1
+ | EVar v => 1
+ | EFunId f => 1
+ | EFun vl e => 1 + size e
+ | ERecFun f vl e => 1 + size e
+ | EApp exp l => 1 + size exp + fold_right (fun x acc => size x + acc) 0 l
+ | ELet v e1 e2 => 1 + size e1 + size e2
+ | ELetRec f vl b e => 1 + size b + size e
+ | EPlus e1 e2 => 1 + size e1 + size e2
+ | EIf e1 e2 e3 => 1 + size e1 + size e2 + size e3
+end.
+
+Definition equiv_exp : Exp -> Exp -> Prop :=
+  fun e1 e2 =>
+  forall env env', equiv_env env env'
+ ->
+  E_rel (v_rel (size e1 + size e2)) env env' e1 e2.
+
+Section examples.
+
+Goal
+  equiv_exp (ELit 5) (EPlus (ELit 5) (ELit 0)).
+Proof.
+  unfold equiv_exp. intros.
+  constructor.
+  * prove_term.
+  * intros. destruct H0, clock; inversion H0. destruct clock; inversion H1. repeat constructor.
+Qed.
+
+Goal
+  equiv_exp (EFun [] (ELit 1)) (EFun [] (EPlus (ELit 0) (ELit 1))).
+Proof.
+  start_equiv. prove_term.
+  intros. destruct H0. destruct clock; inversion H0. inversion H1. subst.
+  constructor. intros. auto. simpl.
+  intros. apply length_zero_iff_nil in H2. apply length_zero_iff_nil in H3. subst.
+  constructor. prove_term.
+  intros. destruct H2.
+  destruct clock0; inversion H2. destruct clock0; inversion H3. constructor.
+Qed.
+
+End examples.
+
+Theorem v
+
+(*
+(** Values at base type are V-related exactly when they are identical *)
+Definition V_rel_real : relation (val ℝ) := eq. *)
+
+(*
+(** Values at arrow type are V-related when they take V-related inputs to
+    E-related outputs. *)
+Inductive V_rel_arrow τa τr
+          (V_rel_a : relation (val τa))
+          (V_rel_r : relation (val τr))
+  : relation (val (τa ~> τr)) :=
+| mk_V_rel_arrow (body0 body1 : expr (τa :: ·) τr) :
+    (forall (va0 va1 : val τa),
+        V_rel_a va0 va1 ->
+        E_rel' τr V_rel_r
+               (proj1_sig (ty_subst1 body0 va0))
+               (proj1_sig (ty_subst1 body1 va1))) ->
+      V_rel_arrow τa τr V_rel_a V_rel_r
+                  (v_lam body0)
+                  (v_lam body1).
+Arguments mk_V_rel_arrow {_ _ _ _ _ _} Hva.
+
+(** [V_rel] can't be defined as an inductive without angering the positivity
+    checker. Instead, it is defined in pieces by type, then assembled by
+    fixpoint. *)
+Fixpoint V_rel τ : relation (val τ) :=
+  match τ with
+  | ℝ => V_rel_real
+  | τa ~> τr => V_rel_arrow τa τr (V_rel τa) (V_rel τr)
+  end.
+
+
+*)
+
+
+
